Updated the HTML docs.

src/Phaser.v
@@ -5,7 +5,11 @@ Require Import Vars.
 
 Import Map_TID.
 
+(** A phaser is a map from tasks to phase numbers. *)
+
 Definition phaser := t nat.
+
+(** Operation advance increments the phase of the given task. *)
 
 Definition advance (ph:phaser) (t:tid) : phaser :=
   match find t ph with
@@ -13,29 +17,45 @@ Definition advance (ph:phaser) (t:tid) : phaser :=
     | None => ph
   end.
 
+(** Operation await holds when every member of the phaser has
+    reached at least phase [n]. *)
+
 Definition await (ph:phaser) (n:nat) : Prop :=
   forall t n',
   MapsTo t n' ph ->
   n' <= n.
 
+(** Operation [register] assigns a new member in the phaser. *)
+
 Definition register (ph:phaser) (t:tid) (n:nat) : phaser :=
   add t n ph.
+
+(** Operation [deregister] revokes the membership of a task in the phaser. *)
 
 Definition deregister (ph:phaser) (t:tid) : phaser :=
   remove t ph.
 
+(** Operation [phase] looks up the phase associated with a given task,
+    or yields [None] if the given task  is unregistered. *)
+
 Definition phase (ph:phaser) (t:tid) : option nat :=
   find t ph.
 
+(** Creates a phaser with a given task initialized at phase [0]. *)
+
 Definition make (t:tid) : phaser :=
   add t 0 (empty nat).
+
+(** Defines the API of a phaser. *)
 
 Inductive op :=
   | ADV : op
   | REG : tid -> op
   | DEREG : op.
 
-Definition apply (ph:phaser) (t:tid) (o:op) : phaser :=
+(** Applies a phaser operation according to the tag. *)
+
+Definition eval (ph:phaser) (t:tid) (o:op) : phaser :=
   match o with
     | ADV => advance ph t
     | REG t' =>
