src/PhaserMap.v
@@ -4,26 +4,42 @@ Require Import Coq.Structures.OrderedTypeEx.
 Require Import Phaser.
 Require Import Vars.
 
-(* Define types *)
+(** A phaser map is a map from phaser identifier to a [phaser] state. *)
+
 Import Map_PHID.
 Definition phasermap := t phaser.
 
-(* Define operations. *)
+(** Function [make] creates an empty phasermap. *)
+
 Definition make := empty phaser.
+
+(** Function [newPhaser pm t p] expects a phaser map [pm] a task identifier [t]
+  and a phaser identifier [p] and assigns a new phaser state to identifier [p];
+  the phaser state is registered with task [t], as per [Phaser.make]. *)
+
 Definition newPhaser (pm:phasermap) (t:tid) (p:phid) : phasermap :=
   add p (Phaser.make t) pm.
+
+(** Thus, there are two possible operations, either we create a phaser
+  with [NEW] or we invoke a phaser operation with [APP]. *)
 
 Inductive op :=
   | NEW : phid -> op
   | APP : phid -> Phaser.op -> op.
 
+(** Function [ph_apply pm t p o] looks up the phaser associated with
+identifier [p] and applies a phaser operation [o] to that phaser, prefixed
+with task [t]. *)
+
 Definition ph_apply (pm:phasermap) (t:tid) (p:phid) (o:Phaser.op) : phasermap :=
   match find p pm with
-    | Some ph => add p (Phaser.apply ph t o) pm
+    | Some ph => add p (Phaser.eval ph t o) pm
     | None => pm
   end.
 
-Definition apply (pm:phasermap) (t:tid) (o:op) : phasermap :=
+(** The semantics can be summarized with operation [eval]. *)
+
+Definition eval (pm:phasermap) (t:tid) (o:op) : phasermap :=
   match o with
     | NEW p => newPhaser pm t p
     | APP p o' => ph_apply pm t p o'
