src/Example1.v
@@ -11,23 +11,21 @@ Definition bd := LOOP(bl) ;; DEREG(ph1);; END.
 Definition b := ph1 <- NEW_PHASER;; bd.
 Definition s1_tm := TaskMap.add td b TaskMap.make.
 
-(* The initial state uses the load function. *)
+(** Initializes an abstract state from a program. *)
 Definition s1 := load td b.
 
+(** Performs the first reduction step that creates a phaser. *)
 Definition s2_td := bd.
 Definition s2_tm := add td s2_td s1_tm.
-Definition s2_pm := PhaserMap.apply PhaserMap.make td (PhaserMap.NEW ph1).
+Definition s2_pm := PhaserMap.eval PhaserMap.make td (PhaserMap.NEW ph1).
 Definition s2 :state := (s2_pm, s2_tm).
 Lemma td_In_s1_tm : TaskMap.MapsTo td b s1_tm.
-assert (H: TID.eq td td).
-apply (TID.eq_refl td).
-apply Map_TID.add_1.
-assumption.
+  assert (H: TID.eq td td) by apply (TID.eq_refl td).
+  apply Map_TID.add_1; auto.
 Qed.
 
-Goal s_redex s1 s2.
-assert (H:=RPhaser (PhaserMap.NEW ph1) td bd PhaserMap.make s1_tm td_In_s1_tm).
-auto.
+Goal Reduces s1 s2.
+  eauto using r_phaser, PhaserMap.make, s1_tm, td_In_s1_tm.
 Qed.
 
 Definition s3_td := t1 <- NEW_TID;; REG(ph1, t1);; FORK(t1, bf);; bd.
@@ -35,13 +33,13 @@ Definition s3_tm := TaskMap.add td s3_td s2_tm.
 Definition s3_pm := s2_pm.
 Definition s3 :state := (s3_pm, s3_tm).
 
-Goal s_redex s2 s3.
-apply RCFlow with (c:=loop bl) (p:=DEREG(ph1);; END).
-unfold s2_tm.
-unfold s2_td.
-unfold bd.
-apply Map_TID.add_1.
-apply (TID.eq_refl td).
-apply RIter with (p:=bl) (q:=((DEREG  (ph1));; END)).
+(** The next reduction step is to unfold the loop. *)
+Goal Reduces s2 s3.
+  apply r_cflow with (c:=loop bl) (p:=DEREG(ph1);; END).
+  - unfold s2_tm.
+    unfold s2_td.
+    unfold bd.
+    apply Map_TID.add_1; auto using TID.eq_refl.
+  - eapply ControlFlow.r_iter; eauto.
 Qed.
 
