src/TaskMap.v
@@ -3,9 +3,16 @@ Require Import Vars.
 
 Import Map_TID.
 
+(** A task map is a map from task identifiers to programs. *)
+
 Definition taskmap := t prog.
 
+(** Function [make] creates an empty task map. *)
+
 Definition make : taskmap := empty prog.
+
+(** Function [newTask t tm] puts a task identifier [t] in the task map [tm] 
+    initialized with an empty program. *)
 
 Definition newTask (tm:taskmap) (t:tid) : taskmap :=
   add t pnil tm.
